Add a semi-automatic derivation of the Bookstore example

examples/BookstoreSemiAutomatic.v
@@ -1,4 +1,4 @@
-Require Import AutoDB.
+ Require Import AutoDB.
 
 (* Our bookstore has two relations (tables):
    - The [Books] relation contains the books in the
@@ -118,16 +118,108 @@ Definition BookStore_AbsR
            (nr : TBookStorage * TOrderStorage) : Prop :=
   or!sBOOKS ≃ benumerate (fst nr) /\ or!sORDERS ≃ benumerate (snd nr).
 
-(* An efficient implementation for the bookstore example can be
-   obtained in a fully automated manner using our query planner,
-   which should take anywhere from 10 to 25 minutes to complete *)
-Definition BookStore :
-  Sharpened BookStoreSpec.
-Proof. 
-  plan BookStore_AbsR.
+Definition BookStoreManual : 
+  Sharpened BookStoreSpec.  
+Proof.
+  unfold BookStoreSpec.
+  
+  (* First, we unfold various definitions and drop constraints *)
+  start honing QueryStructure.
+
+  (* Then we introduce the BookStore_AbsR abstraction relation *)
+  hone representation using BookStore_AbsR.
+
+  (* We start the actual refinement with the constructor, in a fully
+  automated way *) 
+  hone constructor "Init". { 
+    initializer. 
+  }
+
+  (* We then move on to the "PlaceOrder" method, which we decide to 
+     implement semi-manually *)
+  hone method "PlaceOrder". {
+    (* First, we unfold the definition of our abstraction relation *) 
+    startMethod BookStore_AbsR. 
+    
+    (* The, we remove trivial or redundant checks *)
+    pruneDuplicates.
+
+    (* Since the specification represents datasets as mathematical
+       sets, every inserted item is paired with a unique ID, which we
+       need to pick. Further refinements will drop this index, which
+       thus doesn't have any computational cost. *) 
+    pickIndex.
+
+    (* To ease its implementation, we convert this foregin key check
+       into a query *) 
+    foreignToQuery.
+    
+    (* This query, operating on sets, is then transformed into a
+       filter on lists, making use of the equivalence relations 
+       specified by Bookstore_AbsR *)
+    concretize.
+
+    (* At this point, we need to pick a list of results whose elements
+       are a permutation of the one derived from the query. Using
+       permutation-preserving transformations, we substitute slow
+       operations for more efficient ones *) 
+    asPerm (BookStorage, OrderStorage).
+    
+    (* This representation is reasonnably satisfactory; we pick the
+       resulting list, and proceed to a few extra optimizations *)
+    commit.
+
+    (* Now that we have a decision procedure for the constraint checks, 
+       all that remains is to proceed to the actual insertions. We 
+       distinguish the case where checks succeeded, and the case where 
+       checks failed. *)
+    Split Constraint Checks.
+
+    (* First, the case where checks succeed: the insertion is valid: *)
+    checksSucceeded.
+
+    (* Second, the case where checks failed: in that case, the DB
+       remains untouched: *)
+    checksFailed.
+  }
+
+  (* The AddBook method follows a similar pattern, so we implement it
+      automatically: *)
+  hone method "AddBook". {
+    mutator.
+  }
+
+  (* We then move on to implementing the observers. First, GetTitles;
+     again, we adopt a slightly more manual style to demonstrate the
+     main steps of the implementation. *) 
+  hone method "GetTitles". {
+    (* Just as before, we unfold the definition of our abstraction
+       relation *) 
+    startMethod BookStore_AbsR.
+
+    (* And just like before, we translate this query in terms of list
+       operations. *) 
+    concretize.
+ 
+    (* The optimization of this query follows a similar pattern: *)
+    asPerm BookStorage.
+
+    (* This optimization is satisfactory: we pick the resulting list *) 
+    commit.
+
+    (* GetTitles is an observer: it doesn't modify the tables in any way. *)
+    choose_db BookStore_AbsR.
+
+    (* And we're done! *)
+    finish honing.
+  }
+
+  (* Our last method is NumOrders, which we can pass to the automatic
+  query planner. This takes a few minutes to complete *) 
+  hone method "NumOrders". {
+    observer.
+  }
+
+  (* At this point our implementation is fully computational: we're done! *)
   finish sharpening.
 Defined.
-
-(* The same implementation can of course be derived in a more manual
-way; the derivation in BookstoreSemiAutomatic.v demonstrates such an
-implementation, using varying degrees of automation for each method *)
